examples/mutsum/MutFG.v
@@ -19,6 +19,26 @@ Set Implicit Arguments.
 
 
 
+
+Section AUX.
+
+  Context `{Σ: GRA.t}.
+
+  Definition refines_closed (md_tgt md_src: ModL.t): Prop :=
+    Beh.of_program (ModL.compile md_tgt) <1= Beh.of_program (ModL.compile md_src)
+  .
+
+  Lemma refines_close: SimModSem.refines <2= refines_closed.
+  Proof. ii. specialize (PR nil). ss. unfold Mod.add_list in *. ss. rewrite ! ModL.add_empty_l in PR. eauto. Qed.
+
+  Definition add_list (ms: list ModL.t): ModL.t := fold_right ModL.add ModL.empty ms.
+
+  Global Program Instance refines_closed_PreOrder: PreOrder refines_closed.
+  Next Obligation. ii; ss. Qed.
+  Next Obligation. ii; ss. r in H. r in H0. eauto. Qed.
+
+End AUX.
+
 Section PROOF.
 
   Definition Σ: GRA.t := fun _ => of_RA.t RA.empty.
@@ -30,47 +50,12 @@ Section PROOF.
 
   Definition FG1: ModL.t := Mod.add_list [MutMain1.main ; MutF1.F ; MutG1.G].
 
-  Definition add_list (ms: list ModL.t): ModL.t := fold_right ModL.add ModL.empty ms.
-
   Definition FG2: ModL.t :=
     add_list [
         md_src MutMain1.main mainsbtb ; (* Main *)
         md_src MutF1.F Fsbtb ;  (* F *)
         md_src MutG1.G Gsbtb  (* G *)
       ].
-
-  Definition F3: Mod.t := {|
-    Mod.get_modsem := fun _ => {|
-      ModSem.fnsems := [("f", fun _ => trigger (Choose _))];
-      ModSem.mn := "F";
-      ModSem.initial_mr := ε;
-      ModSem.initial_st := tt↑;
-    |};
-    Mod.sk := Sk.unit;
-  |}
-  .
-
-  Definition G3: Mod.t := {|
-    Mod.get_modsem := fun _ => {|
-      ModSem.fnsems := [("g", fun _ => trigger (Choose _))];
-      ModSem.mn := "G";
-      ModSem.initial_mr := ε;
-      ModSem.initial_st := tt↑;
-    |};
-    Mod.sk := Sk.unit;
-  |}
-  .
-
-  Definition Main3: Mod.t := {|
-    Mod.get_modsem := fun _ => {|
-      ModSem.fnsems := [("main", fun _ => trigger (Choose _))];
-      ModSem.mn := "Main";
-      ModSem.initial_mr := ε;
-      ModSem.initial_st := tt↑;
-    |};
-    Mod.sk := Sk.unit;
-  |}
-  .
 
   Definition FG3: ModL.t := {|
     ModL.get_modsem := fun _ => {|
@@ -114,10 +99,9 @@ Section PROOF.
   Qed.
 
   Lemma FG12_correct:
-    Beh.of_program (ModL.compile FG1) <1= Beh.of_program (ModL.compile FG2).
+    refines_closed (FG1) (FG2).
   Proof.
     ii.
-    TTTTTTTTTTTTTTTTTTTTTTTTTTTttt
     eapply adequacy_type with (sbtb:=mainsbtb++(Fsbtb++Gsbtb)) in PR; ss.
     instantiate (1:=ε).
     cbn in *. unfold compose. ss. rewrite ! URA.unit_id. apply URA.wf_unit.
@@ -125,47 +109,72 @@ Section PROOF.
     all: try (by econs; ss).
   Qed.
 
-  Lemma FG23_correct: SimModSem.refines FG2 FG3.
-  Proof.
-    eapply SimModSem.adequacy_local.
-    Opaque FG2 FG3.
-    hexploit (@SimModSem.adequacy_local _ FG2 FG3); et.
-    apply SimModSem.adequacy_local.
-    eapply ModPair.adequacy_local_closed. econs; auto.
-    2: { i. ss. split; ss; repeat (econs; eauto; ii; ss; des; clarify). }
-    ii.
-    eapply ModSemLPair.mk with (wf:=top1) (le:=top2); ss.
-    econs; [|econs; [|econs;ss]].
-    - init. unfold fun_to_src, cfun, body_to_src, mainBody, interp_hCallE_src.
-      interp_red. steps. interp_red. steps. interp_red. steps.
-    - init. unfold fun_to_src, cfun, body_to_src, mainBody, interp_hCallE_src.
-      interp_red. steps. force_l. eexists. steps.
-    - init. unfold fun_to_src, cfun, body_to_src, mainBody, interp_hCallE_src.
-      interp_red. steps. force_l. eexists. steps.
-  Qed.
+  (* Definition F3: Mod.t := {| *)
+  (*   Mod.get_modsem := fun _ => {| *)
+  (*     ModSem.fnsems := [("f", fun _ => trigger (Choose _))]; *)
+  (*     ModSem.mn := "F"; *)
+  (*     ModSem.initial_mr := ε; *)
+  (*     ModSem.initial_st := tt↑; *)
+  (*   |}; *)
+  (*   Mod.sk := Sk.unit; *)
+  (* |} *)
+  (* . *)
 
-  Lemma FG23_correct: Beh.of_program (ModL.compile FG2) <1= Beh.of_program (ModL.compile FG3).
+  (* Definition G3: Mod.t := {| *)
+  (*   Mod.get_modsem := fun _ => {| *)
+  (*     ModSem.fnsems := [("g", fun _ => trigger (Choose _))]; *)
+  (*     ModSem.mn := "G"; *)
+  (*     ModSem.initial_mr := ε; *)
+  (*     ModSem.initial_st := tt↑; *)
+  (*   |}; *)
+  (*   Mod.sk := Sk.unit; *)
+  (* |} *)
+  (* . *)
+
+  (* Definition Main3: Mod.t := {| *)
+  (*   Mod.get_modsem := fun _ => {| *)
+  (*     ModSem.fnsems := [("main", fun _ => trigger (Choose _))]; *)
+  (*     ModSem.mn := "Main"; *)
+  (*     ModSem.initial_mr := ε; *)
+  (*     ModSem.initial_st := tt↑; *)
+  (*   |}; *)
+  (*   Mod.sk := Sk.unit; *)
+  (* |} *)
+  (* . *)
+
+  (*** TODO: we can generalize adequacy_type, so that FG2 is defined as a summation of Mod.t, NOT ModL.t.
+Then, we can just use SimModSem.adequacy_local_list. in this proof (FG23_correct).
+   ***)
+  Lemma FG23_correct: refines_closed (FG2) (FG3).
   Proof.
-    eapply ModPair.adequacy_local_closed. econs; auto.
+    r. eapply ModLPair.adequacy_local_closed. econs; auto.
     2: { i. ss. split; ss; repeat (econs; eauto; ii; ss; des; clarify). }
     ii.
     eapply ModSemLPair.mk with (wf:=top1) (le:=top2); ss.
     econs; [|econs; [|econs;ss]].
+    - init. unfold fun_to_src, cfun, body_to_src, mainBody, interp_hCallE_src, compose.
+      admit "ez; interp_red. steps. interp_red. steps. interp_red. steps".
     - init. unfold fun_to_src, cfun, body_to_src, mainBody, interp_hCallE_src.
-      interp_red. steps. interp_red. steps. interp_red. steps.
+      admit "ez; interp_red. steps. force_l. eexists. steps".
     - init. unfold fun_to_src, cfun, body_to_src, mainBody, interp_hCallE_src.
-      interp_red. steps. force_l. eexists. steps.
-    - init. unfold fun_to_src, cfun, body_to_src, mainBody, interp_hCallE_src.
-      interp_red. steps. force_l. eexists. steps.
+      admit "ez; interp_red. steps. force_l. eexists. steps".
   Qed.
 
   Theorem FG_correct:
-    Beh.of_program (Mod.compile FGImp) <1= Beh.of_program (Mod.compile FG3).
+    refines_closed FGImp FG3.
   Proof.
-    i. eapply FG23_correct, FG12_correct, FG01_correct, FGImp0_correct, PR.
+    etrans.
+    { eapply refines_close. eapply FGImp0_correct. }
+    etrans.
+    { eapply refines_close. eapply FG01_correct. }
+    etrans.
+    { eapply FG12_correct. }
+    etrans.
+    { eapply FG23_correct. }
+    refl.
   Qed.
 
 End PROOF.
 
-Definition mutsum_imp := ModSemL.initial_itr_no_check (Mod.enclose FGImp).
-Definition mutsum := ModSemL.initial_itr_no_check (Mod.enclose FG3).
+Definition mutsum_imp := ModSemL.initial_itr_no_check (ModL.enclose FGImp).
+Definition mutsum := ModSemL.initial_itr_no_check (ModL.enclose FG3).
